src/Init/Prelude.lean
@@ -291,7 +291,7 @@ the statement of the theorem is `a = a`, Lean will allow anything that is
 definitionally equal to that type. So, for instance, `2 + 2 = 4` is proven in
 Lean by `rfl`, because both sides are the same up to definitional equality.
 -/
-@[match_pattern] def rfl {α : Sort u} {a : α} : Eq a a := Eq.refl a
+@[match_pattern] theorem rfl {α : Sort u} {a : α} : Eq a a := Eq.refl a
 
 /-- `id x = x`, as a `@[simp]` lemma. -/
 @[simp] theorem id_eq (a : α) : Eq (id a) a := rfl
@@ -458,7 +458,7 @@ inductive HEq : {α : Sort u} → α → {β : Sort u} → β → Prop where
   | refl (a : α) : HEq a a
 
 /-- A version of `HEq.refl` with an implicit argument. -/
-@[match_pattern] protected def HEq.rfl {α : Sort u} {a : α} : HEq a a :=
+@[match_pattern] protected theorem HEq.rfl {α : Sort u} {a : α} : HEq a a :=
   HEq.refl a
 
 theorem eq_of_heq {α : Sort u} {a a' : α} (h : HEq a a') : Eq a a' :=
@@ -740,7 +740,7 @@ prove `p` given any element `x : α`, then `p` holds. Note that it is essential
 that `p` is a `Prop` here; the version with `p` being a `Sort u` is equivalent
 to `Classical.choice`.
 -/
-protected def Nonempty.elim {α : Sort u} {p : Prop} (h₁ : Nonempty α) (h₂ : α → p) : p :=
+protected theorem Nonempty.elim {α : Sort u} {p : Prop} (h₁ : Nonempty α) (h₂ : α → p) : p :=
   match h₁ with
   | intro a => h₂ a
 
@@ -3150,7 +3150,7 @@ instance (ρ : Type u) (m : Type u → Type v) [MonadWithReaderOf ρ m] : MonadW
 instance {ρ : Type u} {m : Type u → Type v} {n : Type u → Type v} [MonadFunctor m n] [MonadWithReaderOf ρ m] : MonadWithReaderOf ρ n where
   withReader f := monadMap (m := m) (withTheReader ρ f)
 
-instance {ρ : Type u} {m : Type u → Type v} [Monad m] : MonadWithReaderOf ρ (ReaderT ρ m) where
+instance {ρ : Type u} {m : Type u → Type v} : MonadWithReaderOf ρ (ReaderT ρ m) where
   withReader f x := fun ctx => x (f ctx)
 
 /--
@@ -3233,7 +3233,7 @@ def modify {σ : Type u} {m : Type u → Type v} [MonadState σ m] (f : σ → �
 of the state. It is equivalent to `get <* modify f` but may be more efficient.
 -/
 @[always_inline, inline]
-def getModify {σ : Type u} {m : Type u → Type v} [MonadState σ m] [Monad m] (f : σ → σ) : m σ :=
+def getModify {σ : Type u} {m : Type u → Type v} [MonadState σ m] (f : σ → σ) : m σ :=
   modifyGet fun s => (s, f s)
 
 -- NOTE: The Ordering of the following two instances determines that the top-most `StateT` Monad layer
