src/Lean/Environment.lean
@@ -599,7 +599,7 @@ end TagDeclarationExtension
 
 def MapDeclarationExtension (α : Type) := SimplePersistentEnvExtension (Name × α) (NameMap α)
 
-def mkMapDeclarationExtension [Inhabited α] (name : Name := by exact decl_name%) : IO (MapDeclarationExtension α) :=
+def mkMapDeclarationExtension (name : Name := by exact decl_name%) : IO (MapDeclarationExtension α) :=
   registerSimplePersistentEnvExtension {
     name          := name,
     addImportedFn := fun _ => {},
